%  This is a LaTex file.

%  Homework for the course "AMath 585:  Applied Linear Algebra and Numerical Analysis",
%  Autumn quarter, 2009, Anne Greenbaum.


%   A latex format for making homework assignments.


\documentclass[letterpaper,12pt]{article}

%          The page format, somewhat wider and taller page than in art12.sty.

\topmargin -0.1in \headsep 0in \textheight 8.9in \footskip 0.6in
\oddsidemargin 0in  \evensidemargin 0in  \textwidth 6.5in
\usepackage{graphicx}
\usepackage{listings}
\usepackage{caption}
\usepackage{subcaption}
\usepackage{color}
\usepackage{float}
\definecolor{keywords}{RGB}{255,0,90}
\definecolor{comments}{RGB}{0,0,113}
\definecolor{red}{RGB}{160,0,0}
\definecolor{green}{RGB}{0,150,0}
\definecolor{codegreen}{rgb}{0,0.6,0}
\definecolor{codegray}{rgb}{0.5,0.5,0.5}
\definecolor{codepurple}{rgb}{0.58,0,0.82}
\definecolor{backcolour}{rgb}{0.95,0.95,0.92}
\definecolor{brown}{rgb}{0.59, 0.29, 0.0}
\definecolor{beaublue}{rgb}{0.74, 0.83, 0.9}
\definecolor{orange}{rgb}{1.0, 0.5, 0.0}
\definecolor{darkslategray}{rgb}{0.18, 0.31, 0.31}
\definecolor{deepblue}{rgb}{0,0,0.5}
\definecolor{deepred}{rgb}{0.6,0,0}
\definecolor{deepgreen}{rgb}{0,0.5,0}
\lstdefinestyle{myMatlabstyle}{
	language=Matlab,
	backgroundcolor=\color{white},
	commentstyle=\color{codegreen},
	keywordstyle=\color{blue},
	%identifierstyle=\color{brown},
	numberstyle=\tiny\color{codegray},
	stringstyle=\color{orange},
	basicstyle=\footnotesize,
	breakatwhitespace=false,
	breaklines=true,
	captionpos=b,
	keepspaces=true,
	numbers=left,
	numbersep=5pt,
	showspaces=false,
	showstringspaces=false,
	showtabs=false,
	tabsize=2
}
\lstdefinestyle{myPythonstyle}{
	language=Python,
	basicstyle=\ttfamily\small,
	keywordstyle=\color{blue},
	backgroundcolor=\color{white},
	commentstyle=\color{green},
	stringstyle=\color{red},
	showstringspaces=false,
	%identifierstyle=\color{brown},
	breaklines=true,
}
\lstset{language=Matlab,frame=single}
\lstset{language=Python,frame=single}
\usepackage{amsmath}
\usepackage{epsfig}         % to insert PostScript figures
       % to insert PostScript figures

\begin{document}


%          Definitions of commonly used symbols.



%          The title and header.

\noindent
{\scriptsize ES$\_$APPM 411-1, Fall 2018} \hfill

\begin{center}
\large
Assignment 1.
\normalsize

Jithin D. George
\end{center}

\noindent
Due Oct 2
\vspace{.3in}

%           The questions!



\noindent


\begin{enumerate}
\item
\[x^2y' +(1+x^2)y =0\]
\[\frac{y'}{y} = -1- \frac{1}{x^2}\]
\[\log(y)= -x+\frac{1}{x}+C\]
\[y = Ae^{\frac{1}{x}-x}\]
\item
\[xy' + 3y=-x\]
Multiplying by the integrating factor,
\[x^3y' + 3x^2y=-x^3\]
\[(x^3y)'=-x^3\]
\[x^3y=-\frac{x^4}{4}+C\]
\[y=-\frac{x}{4}+\frac{C}{x^3}\]
\item
\[y'' +6y' +5y=0\]
Using the ansatz $e^{mx}$,
\[m^2e^{mx} + 6me^{mx}+5e^{mx}=0 \]
\[m^2 + 6m+5=0 \]
\[m = -1,-5\]
Thus,
\[y = c_1 e^{-x}+c_2 e^{-5x}\]
\item
\[y'' +6y' +9y=0\]
Using the ansatz $e^{mx}$,
\[m^2e^{mx} + 6me^{mx}+9e^{mx}=0 \]
\[m^2 + 6m+9=0 \]
\[m = -3,-3\]
Since the root is repeated, we can use reduction of order to find that the general solution is
\[y = c_1 e^{-3x}+c_2 xe^{-3x}\]
\item
\[y'' +6y' +13y=0\]
Using the ansatz $e^{mx}$,
\[m^2e^{mx} + 6me^{mx}+13e^{mx}=0 \]
\[m^2 + 6m+13=0 \]
\[m = -3+2i,-3-2i\]
Since the root are complex, the general solution is
\[y = e^{-3x}(c_1 sin(2x)+ c_2 cos(2x))\]

\item
\[y'''+y''-y'-y=0\]

Using the ansatz $e^{mx}$,
\[m^3e^{mx}+m^2e^{mx} -me^{mx}-e^{mx}=0 \]
\[m^3+m^2 -m-1=0 \]
\[(m^2-1)(m+1)=1\]
\[m = 1,-1,-1\]
Since e $-1$ is repeated twice, the general solution is
\[y = c_1 e^{x}+ c_2 e^{-x}+c_3 xe^{-x}\]

\item
\[xy'' + 3y'=x^2\]
Multiplying by the integrating factor,
\[x^3y'' + 3x^2y'=x^4\]
\[(x^3y')'=x^4\]
\[x^3y'=\frac{x^5}{5}+c_1\]
\[y'=\frac{x^2}{5}+\frac{C}{x^3}\]
\[y =\frac{x^3}{15}-\frac{c_1}{2x^2}+c_2\]
\item
\[(x-1)y''-xy'+y=0\]
Plugging in $y_2 = u(x)y_1$, we get
\[(x-1)(u''y_1 +2u'y_1'+uy_1'')-x(u'y_1+uy_1')+uy_1=0\]
\[(x-1)(u''y_1 +2u'y_1')-x(u'y_1)=0\]
\[(x-1)(u''e^{x} +2u'e^x)-x(u'e^x)=0\]
\[(x-1)u''+ (x-2)u'=0\]
\[\frac{u''}{u'}=-\frac{x-2}{x-1}= -1 + \frac{1}{x-1}\]
\[\log(u')= c_1-x +log(x-1)\]
\[u'= c_1(x-1)e^{-x}\]
\[u= c_1xe^{-x} +c_2\]
\[y = uy_1 = c_1 x + c_2 e^x\]
\end{enumerate}
\end{document}
